Definedness_Normalization/Definedness_Normalization_Semantics.thy
@@ -1,0 +1,280 @@
+theory Definedness_Normalization_Semantics
+  imports Definedness_Normalization
+begin
+
+section ‹Definedness Explication Preserves Semantics›
+
+subsection ‹Helper lemmas on ‹foldr (❙∧) (map Atom _)››
+
+lemma foldr_and_imp_orig:
+  assumes "𝒜 ⊨⇩m foldr (❙∧) (map Atom as) F"
+  shows "𝒜 ⊨⇩m F"
+  using assms by (induction as) auto
+
+lemma foldr_and_if:
+  assumes "𝒜 ⊨⇩m F"
+      and "∀a ∈ set as. 𝒜 a = Some True"
+    shows "𝒜 ⊨⇩m foldr (❙∧) (map Atom as) F"
+  using assms by (induction as) auto
+
+subsection ‹Definedness atoms under a defined-PNE valuation›
+
+lemma definedness_atom_valuation:
+  assumes "atoms F ⊆ dom (valuation M)"
+      and "a ∈ set (definedness_atoms F)"
+    shows "valuation M a = Some True"
+proof -
+  from assms(2) obtain p where p:
+    "p ∈ set (formula_enumerate_primitive_numeric_expressions F)"
+    "a = numericEqAtm (FunctionExpr p) (FunctionExpr p)"
+    by (rule definedness_atoms_form)
+  from p(1) assms(1) have "p ∈ dom (snd M)"
+    using formula_atoms_in_dom_valuation_iff by fast
+  thus ?thesis unfolding p(2) valuation_def by (cases "snd M p") auto
+qed
+
+lemma definedness_atoms_subset_dom_valuation:
+  assumes "atoms F ⊆ dom (valuation M)"
+  shows "set (definedness_atoms F) ⊆ dom (valuation M)"
+  using definedness_atom_valuation[OF assms] by (auto simp: domIff)
+
+subsection ‹Key semantic equivalence›
+
+theorem explicate_def_fmla_semantics:
+  "valuation M ⊨⇩m explicate_def_fmla f ⟷ valuation M ⊨⇩m f"
+proof
+  assume "valuation M ⊨⇩m explicate_def_fmla f"
+  thus "valuation M ⊨⇩m f"
+    unfolding explicate_def_fmla_def using foldr_and_imp_orig by blast
+next
+  assume sat: "valuation M ⊨⇩m f"
+  hence atoms_in: "atoms f ⊆ dom (valuation M)" by blast
+  show "valuation M ⊨⇩m explicate_def_fmla f"
+    unfolding explicate_def_fmla_def
+    by (rule foldr_and_if[OF sat], rule ballI, rule definedness_atom_valuation[OF atoms_in])
+qed
+
+subsection ‹Substitution commutes with explication›
+
+text ‹Needed for the action-instantiation argument: substituting parameters
+  into an explicated precondition yields the same formula as explicating the
+  substituted precondition. The PNE-enumeration map lemmas are inherited from
+  ‹Definedness_Normalization›.›
+
+lemma definedness_atoms_map:
+  "definedness_atoms (map_formula (map_atom m) F)
+    = map (map_atom m) (definedness_atoms F)"
+  unfolding definedness_atoms_def Let_def
+  by (simp add: formula_enumerate_primitive_numeric_expressions_map comp_def)
+
+lemma foldr_and_map:
+  "map_formula (map_atom m) (foldr (❙∧) (map Atom as) f)
+    = foldr (❙∧) (map Atom (map (map_atom m) as)) (map_formula (map_atom m) f)"
+  by (induction as) auto
+
+lemma explicate_def_fmla_map:
+  "map_formula (map_atom m) (explicate_def_fmla f)
+    = explicate_def_fmla (map_formula (map_atom m) f)"
+  unfolding explicate_def_fmla_def
+  by (simp add: foldr_and_map definedness_atoms_map)
+
+subsection ‹Plan-action enabledness is preserved›
+
+context ast_classical_problem_de begin
+
+lemma inst_pre_explicate_def:
+  "ground_action.precondition
+     (instantiate_classical_action_schema (explicate_def_ac a) args)
+   = explicate_def_fmla
+     (ground_action.precondition (instantiate_classical_action_schema a args))"
+  unfolding instantiate_classical_action_schema_alt explicate_def_ac_unfold
+  by (simp add: explicate_def_fmla_map)
+
+lemma inst_pre_iff_explicate_def:
+  "valuation M ⊨⇩m
+     ground_action.precondition (instantiate_classical_action_schema a args)
+   ⟷ valuation M ⊨⇩m
+     ground_action.precondition
+       (instantiate_classical_action_schema (explicate_def_ac a) args)"
+  unfolding inst_pre_explicate_def by (rule explicate_def_fmla_semantics[symmetric])
+
+end
+
+subsection ‹Plan validity is preserved›
+
+text ‹Explication only modifies precondition formulas: action names, parameters,
+  and effects are unchanged. Combined with ‹explicate_def_fmla_semantics›, this
+  lifts to a direct ‹iff› on plan validity. Plan restoration is the identity.›
+
+lemma map_of_pair_map: 
+  "map_of (map (λx. (f x, g x)) xs) n = map_option g (map_of (map (λx. (f x, x)) xs) n)"
+  by (induction xs) auto
+
+context ast_classical_problem_de begin
+
+lemma ast_classical_action_schema_name_explicate [simp]:
+  "ast_classical_action_schema_name (explicate_def_ac a) = ast_classical_action_schema_name a"
+  by (cases a rule: ast_classical_action_schema_cases_unfold) simp
+
+lemma ast_classical_action_schema_head_explicate [simp]:
+  "ast_classical_action_schema_head (explicate_def_ac a) = ast_classical_action_schema_head a"
+  by (cases a rule: ast_classical_action_schema_cases_unfold) simp
+
+lemma d_de_resolve_classical_action_schema:
+  "d_de.resolve_classical_action_schema n
+   = map_option explicate_def_ac (resolve_classical_action_schema n)"
+  unfolding d_de.resolve_classical_action_schema_def resolve_classical_action_schema_def
+            explicate_def_dom_sel index_by_def
+  by (simp add: map_of_pair_map comp_def)
+
+lemma p_de_resolve_classical_action_schema:
+  "p_de.resolve_classical_action_schema n
+   = map_option explicate_def_ac (resolve_classical_action_schema n)"
+  using d_de_resolve_classical_action_schema by simp
+
+lemma p_de_wf_classical_plan_action [simp]:
+  "p_de.wf_classical_plan_action π ⟷ wf_classical_plan_action π"
+proof (cases π)
+  case (SimplePlanAction n args)
+  show ?thesis
+    unfolding SimplePlanAction
+              p_de.wf_classical_plan_action_simple
+              wf_classical_plan_action_simple
+              p_de_resolve_classical_action_schema
+    by (auto split: option.splits)
+qed
+
+lemma p_de_res_inst_precondition:
+  assumes "res_inst π = Some g"
+  shows "∃g'. p_de.res_inst π = Some g'
+    ∧ precondition g' = explicate_def_fmla (precondition g)
+    ∧ effect g' = effect g"
+proof (cases π)
+  case (SimplePlanAction n args)
+  obtain a where res: "resolve_classical_action_schema n = Some a"
+    using assms unfolding SimplePlanAction by (cases "resolve_classical_action_schema n") auto
+  with assms have g_def: "g = instantiate_classical_action_schema a args"
+    unfolding SimplePlanAction by simp
+  have p_de_res: "p_de.res_inst (SimplePlanAction n args)
+    = Some (instantiate_classical_action_schema (explicate_def_ac a) args)"
+    using p_de_resolve_classical_action_schema res by simp
+  have pre_eq: "precondition (instantiate_classical_action_schema (explicate_def_ac a) args)
+    = explicate_def_fmla (precondition g)"
+    using inst_pre_explicate_def[of a args] unfolding g_def by simp
+  have eff_eq: "effect (instantiate_classical_action_schema (explicate_def_ac a) args)
+    = effect g"
+    unfolding g_def instantiate_classical_action_schema_alt by simp
+  show ?thesis using p_de_res pre_eq eff_eq SimplePlanAction by blast
+qed
+
+lemma p_de_res_inst_None [simp]:
+  "p_de.res_inst π = None ⟷ res_inst π = None"
+proof (cases π)
+  case (SimplePlanAction n args)
+  show ?thesis
+    unfolding SimplePlanAction p_de.res_inst.simps res_inst.simps
+              p_de_resolve_classical_action_schema
+    by (cases "resolve_classical_action_schema n") auto
+qed
+
+lemma numeric_effects_non_intrf_explicate:
+  assumes "res_inst π = Some g" "p_de.res_inst π = Some g'"
+  shows "p_de.numeric_effects_non_intrf g' = numeric_effects_non_intrf g"
+proof -
+  from p_de_res_inst_precondition[OF assms(1)] assms(2)
+  have "effect g' = effect g" by auto
+  thus ?thesis
+    unfolding numeric_effects_non_intrf_def by simp
+qed
+
+lemma p_de_plan_action_enabled_iff:
+  "p_de.plan_action_enabled π M ⟷ plan_action_enabled π M"
+proof (cases "res_inst π")
+  case None
+  hence "p_de.res_inst π = None" by simp
+  with None show ?thesis
+    unfolding plan_action_enabled_def p_de.plan_action_enabled_def
+    by simp
+next
+  case (Some g)
+  then obtain g' where g':
+      "p_de.res_inst π = Some g'"
+      "precondition g' = explicate_def_fmla (precondition g)"
+      "effect g' = effect g"
+    using p_de_res_inst_precondition by blast
+  have ne: "p_de.numeric_effects_non_intrf g' = numeric_effects_non_intrf g"
+    using numeric_effects_non_intrf_explicate[OF Some g'(1)] .
+  have rhs: "set (ast_effect_enumerate_rhs_primitive_numeric_expressions (effect g'))
+           = set (ast_effect_enumerate_rhs_primitive_numeric_expressions (effect g))"
+    using g'(3) by simp
+  have wfp: "p_de.wf_classical_plan_action π ⟷ wf_classical_plan_action π" by simp
+  have pre_sem: "valuation M ⊨⇩m precondition g' ⟷ valuation M ⊨⇩m precondition g"
+    unfolding g'(2) by (rule explicate_def_fmla_semantics)
+  show ?thesis
+    unfolding plan_action_enabled_def p_de.plan_action_enabled_def
+    unfolding Some g'(1) Let_def option.sel
+    using ne rhs wfp pre_sem by argo
+qed
+
+lemma p_de_execute_plan_action:
+  "p_de.execute_plan_action π M = execute_plan_action π M"
+proof (cases "res_inst π")
+  case None
+  hence "p_de.res_inst π = None" by simp
+  with None show ?thesis
+    unfolding execute_plan_action_def p_de.execute_plan_action_def
+    by simp
+next
+  case (Some g)
+  then obtain g' where g':
+      "p_de.res_inst π = Some g'"
+      "effect g' = effect g"
+    using p_de_res_inst_precondition by blast
+  have "apply_ground_actions [g'] M = apply_ground_actions [g] M"
+    using g'(2) by (cases g; cases g'; simp add: apply_ground_actions_def)
+  thus ?thesis
+    unfolding execute_plan_action_def p_de.execute_plan_action_def
+    unfolding Some g'(1) by simp
+qed
+
+lemma p_de_valid_classical_plan_alt_iff:
+  "p_de.valid_classical_plan_alt M πs M' ⟷ valid_classical_plan_alt M πs M'"
+proof (induction πs arbitrary: M)
+  case Nil show ?case by simp
+next
+  case (Cons π πs)
+  show ?case
+    by (simp add: Cons.IH p_de_plan_action_enabled_iff p_de_execute_plan_action)
+qed
+
+lemma p_de_I [simp]: "p_de.I = I"
+  unfolding p_de.I_def I_def explicate_def_prob_sel by simp
+
+lemma p_de_valid_classical_plan2_iff:
+  "p_de.valid_classical_plan2 πs ⟷ valid_classical_plan2 πs"
+  unfolding p_de.valid_classical_plan2_alt valid_classical_plan2_alt
+  unfolding p_de_valid_classical_plan_alt_iff p_de_I explicate_def_prob_sel
+  by (simp add: explicate_def_fmla_semantics)
+
+theorem explicate_valid_iff:
+  "(∃πs. valid_classical_plan2 πs) ⟷ (∃πs'. p_de.valid_classical_plan2 πs')"
+  using p_de_valid_classical_plan2_iff by blast
+
+theorem explicate_plan_restore:
+  "p_de.valid_classical_plan2 πs ⟹ valid_classical_plan2 (restore_plan_explicate πs)"
+  using p_de_valid_classical_plan2_iff unfolding restore_plan_explicate_def by simp
+
+end
+
+text ‹Code setup.›
+
+lemmas explicate_def_code =
+  definedness_atoms_def
+  explicate_def_fmla_def
+  explicate_def_ac.simps
+  ast_classical_domain.explicate_def_dom_def
+  ast_classical_problem.explicate_def_prob_def
+
+declare explicate_def_code[code]
+
+end
