Precondition_Normalization/Precondition_Normalization_Semantics.thy
@@ -98,37 +98,35 @@ lemma formula_enumerate_primitive_numeric_expressions_map:
     = map (map_primitive_numeric_expression m) (formula_enumerate_primitive_numeric_expressions F)"
   by (induction F) (auto simp: atom_enumerate_primitive_numeric_expressions_map)
 
-lemma pnes_def_checks_map:
-  "pnes_def_checks (map_formula (map_atom m) F) = map (map_atom m) (pnes_def_checks F)"
-  unfolding pnes_def_checks_def Let_def
-  by (simp add: formula_enumerate_primitive_numeric_expressions_map comp_def)
+text \<open> \<open>is_def_explicated_conj\<close> is preserved by atom substitution. The conj-prefix
+  structure is preserved structurally, and the definedness atom for a PNE \<open>p\<close>
+  maps to the definedness atom for \<open>map_primitive_numeric_expression m p\<close>. \<close>
 
-lemma prepend_atoms_to_conj_map:
-  "map_formula (map_atom m) (prepend_atoms_to_conj as f)
-    = prepend_atoms_to_conj (map (map_atom m) as) (map_formula (map_atom m) f)"
-  unfolding prepend_atoms_to_conj_def by (induction as) auto
+lemma conj_atom_prefix_map_formula:
+  "conj_atom_prefix (map_formula h f) = map h (conj_atom_prefix f)"
+  by (induction f rule: conj_atom_prefix.induct) auto
 
-lemma pne_equiv_dnf_list_map:
-  "map (map_formula (map_atom m)) (pne_equiv_dnf_list F)
-    = pne_equiv_dnf_list (map_formula (map_atom m) F)"
-proof -
-  let ?h = "map_formula (map_atom m)"
-  let ?ck = "pnes_def_checks F"
-  have "map ?h (pne_equiv_dnf_list F)
-      = map ?h (map (prepend_atoms_to_conj ?ck) (dnf_list F))"
-    unfolding pne_equiv_dnf_list_def Let_def ..
-  also have "... = map (\<lambda>c. prepend_atoms_to_conj (map (map_atom m) ?ck) (?h c)) (dnf_list F)"
-    by (simp add: prepend_atoms_to_conj_map)
-  also have "... = map (prepend_atoms_to_conj (pnes_def_checks (?h F)) \<circ> ?h) (dnf_list F)"
-    by (simp add: pnes_def_checks_map comp_def)
-  also have "... = map (prepend_atoms_to_conj (pnes_def_checks (?h F))) (map ?h (dnf_list F))"
-    by simp
-  also have "... = map (prepend_atoms_to_conj (pnes_def_checks (?h F))) (dnf_list (?h F))"
-    by (simp add: dnf_list_map)
-  finally show ?thesis unfolding pne_equiv_dnf_list_def Let_def .
+lemma is_def_explicated_conj_map_atom_fmla:
+  assumes "is_def_explicated_conj f"
+  shows "is_def_explicated_conj (map_atom_fmla m f)"
+  unfolding is_def_explicated_conj_def
+proof (intro ballI)
+  fix p' assume "p' \<in> set (formula_enumerate_primitive_numeric_expressions (map_atom_fmla m f))"
+  then obtain p where p:
+    "p \<in> set (formula_enumerate_primitive_numeric_expressions f)"
+    "p' = map_primitive_numeric_expression m p"
+    using formula_enumerate_primitive_numeric_expressions_map[of m f]
+    by (auto simp: comp_def)
+  from p(1) assms have prefix_f:
+    "numericEqAtm (FunctionExpr p) (FunctionExpr p) \<in> set (conj_atom_prefix f)"
+    unfolding is_def_explicated_conj_def by blast
+  have "map_atom m (numericEqAtm (FunctionExpr p) (FunctionExpr p))
+        = numericEqAtm (FunctionExpr p') (FunctionExpr p')"
+    using p(2) by simp
+  with prefix_f show "numericEqAtm (FunctionExpr p') (FunctionExpr p')
+                       \<in> set (conj_atom_prefix (map_atom_fmla m f))"
+    unfolding comp_def conj_atom_prefix_map_formula by force
 qed
-
-(* end map *)
 
 text \<open> \<open>dnf_list\<close> under \<open>map_formula_semantics\<close>. Unlike the total-valuation version, this
   needs every atom of \<open>F\<close> to be in the domain of \<open>\<A>\<close>: \<open>\<Turnstile>\<^sub>m\<close> is \<open>False\<close> on
@@ -163,141 +161,91 @@ next
   thus ?thesis using False by simp
 qed
 
-lemma prepend_atoms_to_conj_imp_orig:
-  assumes  "\<A> \<Turnstile>\<^sub>m prepend_atoms_to_conj as F"
-  shows "\<A> \<Turnstile>\<^sub>m F"
-  using assms by (induction as arbitrary: F) (simp add: prepend_atoms_to_conj_def)+
-
-lemma pne_equiv_dnf_list_imp_dnf_list:
-  assumes "n < length (dnf_list F)"
-    "\<A> \<Turnstile>\<^sub>m (pne_equiv_dnf_list F ! n)"
-  shows "\<A> \<Turnstile>\<^sub>m (dnf_list F ! n)"
-  using assms by (auto simp: pne_equiv_dnf_list_def intro: prepend_atoms_to_conj_imp_orig)
-
-lemma prepend_atoms_to_conj_if:
-  assumes "\<A> \<Turnstile>\<^sub>m F"
-      and "\<forall>a \<in> (set as). \<A> a = Some True"
-  shows "\<A> \<Turnstile>\<^sub>m prepend_atoms_to_conj as F"
-  using assms 
-proof (induction as)
-  case Nil
-  then show ?case by (simp add: prepend_atoms_to_conj_def)
-next
-  case (Cons a as)
-  have "\<A> \<Turnstile>\<^sub>m prepend_atoms_to_conj as F" using prepend_atoms_to_conj_def Cons by auto
-  moreover
-  have "\<A> \<Turnstile>\<^sub>m Atom a" using Cons by simp
-  moreover
-  have "atoms (prepend_atoms_to_conj (a#as) F) \<subseteq> dom \<A>" using Cons by auto
-  ultimately
-  show ?case by (simp add: comp_def prepend_atoms_to_conj_def)
-qed
-
-lemma pnes_def_check_in_valuationI:
-  assumes "atoms F \<subseteq> dom (valuation M)"
-  shows "set (pnes_def_checks F) \<subseteq> dom (valuation M)"
-proof -
-  have "(set (formula_enumerate_primitive_numeric_expressions F) \<subseteq> dom (snd M))" (is "set ?fpnes \<subseteq> _")
-    using assms formula_atoms_in_dom_valuation_iff by simp
-  hence "set (concat (map enumerate_primitive_numeric_expressions (map FunctionExpr ?fpnes))) \<subseteq> dom (snd M)"
-    (is "set (concat (map enumerate_primitive_numeric_expressions ?fnes)) \<subseteq> _")
-    by simp
-  hence "set (concat (map atom_enumerate_primitive_numeric_expressions (map (\<lambda>f. numericEqAtm f f) ?fnes))) \<subseteq> dom (snd M)"
-    by simp
-  hence "set (concat (map atom_enumerate_primitive_numeric_expressions (pnes_def_checks F))) \<subseteq> dom (snd M)"
-    unfolding  pnes_def_checks_def Let_def by simp
-  thus ?thesis using dom_valuation_iff by (cases M) auto
-qed
-
-
-lemma in_dom_snd_iff_valuation_eq: 
+lemma in_dom_snd_iff_valuation_eq:
   assumes "eq_expr = Atom (numericEqAtm (FunctionExpr x) (FunctionExpr x))"
   shows "x \<in> dom (snd M) \<longleftrightarrow> valuation M \<Turnstile>\<^sub>m eq_expr"
   unfolding assms valuation_def by (cases "snd M x") auto
 
-lemma pnes_def_check_valuation_semI:
-  assumes "atoms F \<subseteq> dom (valuation M)"
-      and "c \<in> set (pnes_def_checks F)"
-    shows "valuation M \<Turnstile>\<^sub>m Atom c"
-proof -
-  obtain x where
-    x: "c = numericEqAtm (FunctionExpr x) (FunctionExpr x)"
-    "x \<in> set (formula_enumerate_primitive_numeric_expressions F)" 
-    using assms(2) unfolding pnes_def_checks_def Let_def by auto
-  thus ?thesis 
-    apply (subst in_dom_snd_iff_valuation_eq[symmetric])
-    using assms x formula_atoms_in_dom_valuation_iff assms by auto
-qed
+text \<open> Under \<open>is_def_explicated_conj F\<close>, the semantic equivalence between \<open>F\<close>
+  and its DNF clauses extends to \<open>map_formula_semantics\<close> (no separate
+  definedness-domain side condition needed): every clause of \<open>dnf_list F\<close>
+  enumerates the same PNEs as \<open>F\<close>, so satisfying a clause already forces
+  every PNE of \<open>F\<close> to be defined. \<close>
 
-lemma pne_equiv_dnf_list_atoms_in_valuation_iff:
-  assumes "c \<in> set (pne_equiv_dnf_list F)"
-  shows "atoms F \<subseteq> dom (valuation M) \<longleftrightarrow> atoms c \<subseteq> dom (valuation M)"
-  using assms by (force dest: pne_equiv_dnf_list_pnes simp: formula_atoms_in_dom_valuation_iff)
-
-lemma pne_equiv_dnf_list_map_semantics:
-  "valuation M \<Turnstile>\<^sub>m F \<longleftrightarrow> (\<exists>c\<in>set (pne_equiv_dnf_list F). valuation M \<Turnstile>\<^sub>m c)"
-proof 
-  assume a: "valuation M \<Turnstile>\<^sub>m F"
-
-  have atoms_in_valuation: "atoms F \<subseteq> dom (valuation M)" using a by blast
-  
-  obtain c where
-    c: "c \<in> set (dnf_list F)"
-    "valuation M \<Turnstile>\<^sub>m c" using a dnf_list_map_semantics by metis
-
-  have pne_checks_in_valuation: "set (pnes_def_checks F) \<subseteq> dom (valuation M)"
-    using pnes_def_check_in_valuationI atoms_in_valuation by blast
-
-  have val: "valuation M \<Turnstile>\<^sub>m prepend_atoms_to_conj (pnes_def_checks F) c" 
-    apply (rule prepend_atoms_to_conj_if)
-    apply (rule c(2))
-    using pne_checks_in_valuation pnes_def_check_valuation_semI atoms_in_valuation by simp
-
-  show "\<exists>c\<in>set (pne_equiv_dnf_list F). valuation M \<Turnstile>\<^sub>m c" 
-    using val c unfolding pne_equiv_dnf_list_def by auto
+lemma is_def_explicated_conj_dnf_list_map_semantics:
+  assumes "is_def_explicated_conj F"
+  shows "valuation M \<Turnstile>\<^sub>m F \<longleftrightarrow> (\<exists>c\<in>set (dnf_list F). valuation M \<Turnstile>\<^sub>m c)"
+proof
+  assume "valuation M \<Turnstile>\<^sub>m F"
+  thus "\<exists>c\<in>set (dnf_list F). valuation M \<Turnstile>\<^sub>m c"
+    using dnf_list_map_semantics by metis
 next
-  assume a: "\<exists>c\<in>set (pne_equiv_dnf_list F). valuation M \<Turnstile>\<^sub>m c"
-  obtain c where
-    c: "c \<in> set (pne_equiv_dnf_list F)"
-    "valuation M \<Turnstile>\<^sub>m c" using a by blast
-
-  have atoms_in_val: "atoms F \<subseteq> dom (valuation M)" using pne_equiv_dnf_list_atoms_in_valuation_iff c by blast
-  
-  obtain c' where
-    c': "c = prepend_atoms_to_conj (pnes_def_checks F) c'"
-    "c' \<in> set (dnf_list F)"
-    using c unfolding pne_equiv_dnf_list_def by auto
-
-  have val_sat: "valuation M \<Turnstile>\<^sub>m c'" using c c' prepend_atoms_to_conj_imp_orig by fast
-
-  show "valuation M \<Turnstile>\<^sub>m F" using atoms_in_val val_sat c' dnf_list_map_semantics by blast
+  assume "\<exists>c\<in>set (dnf_list F). valuation M \<Turnstile>\<^sub>m c"
+  then obtain c where c: "c \<in> set (dnf_list F)" "valuation M \<Turnstile>\<^sub>m c" by blast
+  have atoms_c: "atoms c \<subseteq> dom (valuation M)" using c(2) by blast
+  have pnes_eq: "set (formula_enumerate_primitive_numeric_expressions c)
+              = set (formula_enumerate_primitive_numeric_expressions F)"
+    using formula_enum_pnes_dnf_list_def_explicated[OF assms c(1)] .
+  have "atoms F \<subseteq> dom (valuation M)"
+    using atoms_c pnes_eq formula_atoms_in_dom_valuation_iff by metis
+  thus "valuation M \<Turnstile>\<^sub>m F" using c dnf_list_map_semantics by metis
 qed
-
-lemma pne_equiv_dnf_list_conv_dnf_list_map_semantics:
-  "(\<exists>c\<in>set (pne_equiv_dnf_list F). valuation M \<Turnstile>\<^sub>m c)
-  \<longleftrightarrow> (atoms F \<subseteq> dom (valuation M) \<and> (\<exists>c \<in> set (dnf_list F). (valuation M) \<Turnstile>\<^sub>m c))" 
-  apply (subst pne_equiv_dnf_list_map_semantics[symmetric])
-  apply (subst dnf_list_map_semantics)
-  by simp
 
 context ast_classical_domain4 begin
 
-
 lemma precond_prop_iff_split:
-  "(\<exists>c \<in> set (pne_equiv_dnf_list (ac_pre a)). P c) \<longleftrightarrow> (\<exists>a' \<in> set (split_ac a). P (ac_pre a'))"
+  "(\<exists>c \<in> set (dnf_list (ac_pre a)). P c) \<longleftrightarrow> (\<exists>a' \<in> set (split_ac a). P (ac_pre a'))"
 proof -
-  let ?dnf = "pne_equiv_dnf_list (ac_pre a)"
+  let ?dnf = "dnf_list (ac_pre a)"
   have "(\<exists>c \<in> set ?dnf. P c) \<longleftrightarrow> (\<exists>i < length ?dnf. P (?dnf ! i))"
     using in_set_conv_nth by metis
   also have "... \<longleftrightarrow> (\<exists>i < length ?dnf. P (ac_pre (split_ac a ! i)))"
-    using split_ac_nth pne_equiv_dnf_list_map_semantics by auto
+    using split_ac_nth by auto
   also have "... \<longleftrightarrow> (\<exists>a' \<in> set (split_ac a). P (ac_pre a'))"
-    using in_set_conv_nth split_ac_length pne_equiv_dnf_list_length by metis
+    using in_set_conv_nth split_ac_length by metis
   finally show ?thesis by simp
 qed
 
+lemma (in ast_classical_problem4) p_ac_params_match:
+  assumes "a' \<in> set (split_ac a)"
+  shows "action_params_match (head a) = action_params_match (head a')"
+  using split_ac_sel(2)[OF assms] action_params_match_def by presburger
+
+lemma (in ast_classical_problem4) p_effect_same:
+  assumes "b' \<in> set (split_ac b)"
+          "resolve_classical_action_schema n = Some b"
+          "p4.resolve_classical_action_schema n' = Some b'"
+        shows "effect ((the o res_inst) (SimplePlanAction n args)) = effect ((the o p4.res_inst) (SimplePlanAction n' args))"
+  using instantiate_classical_action_schema_alt
+  using split_ac_sel[OF assms(1)] assms(2-) by auto
+
+lemma (in ast_classical_problem4) p_exec:
+  assumes "a' \<in> set (split_ac a)"
+    "resolve_classical_action_schema n = Some a" "p4.resolve_classical_action_schema n' = Some a'"
+  shows "execute_plan_action (SimplePlanAction n args) = p4.execute_plan_action (SimplePlanAction n' args)"
+proof -
+  have "effect ((the o res_inst) (SimplePlanAction n args)) = effect ((the o p4.res_inst) (SimplePlanAction n' args))"
+    using assms p_effect_same by simp
+  hence "apply_ground_actions [(the o res_inst) (SimplePlanAction n args)] =
+    apply_ground_actions [(the o p4.res_inst) (SimplePlanAction n' args)]"
+    using apply_ground_actions_equiv_weak by auto
+  thus ?thesis
+    unfolding ast_classical_problem.execute_plan_action_def
+    by simp
+qed
+
+end
+
+context wf_ast_classical_domain4 begin
+
+text \<open> The semantic equivalence between an action's instantiated precondition
+  and its split clauses uses both the \<open>def_explicated_conj_dom\<close> assumption
+  (every action precondition is conj-prefix definedness-explicated) and the
+  fact that this property is preserved by argument substitution. \<close>
+
 lemma inst_pre_iff_split:
-  shows "valuation M \<Turnstile>\<^sub>m precondition (instantiate_classical_action_schema a args) \<longleftrightarrow> 
+  assumes "a \<in> set (actions D)"
+  shows "valuation M \<Turnstile>\<^sub>m precondition (instantiate_classical_action_schema a args) \<longleftrightarrow>
     (\<exists>a' \<in> set (split_ac a). valuation M \<Turnstile>\<^sub>m precondition (instantiate_classical_action_schema a' args))"
 proof -
   let ?h = "ac_tsubst (ac_params a) args"
@@ -311,16 +259,20 @@ proof -
       = ?inst_fmla (ac_pre a')" if "a' \<in> set (split_ac a)" for a'
     using instantiate_classical_action_schema_alt split_ac_sel(2)[OF that] by simp
 
-  have map_dnf: "pne_equiv_dnf_list (?inst_fmla (ac_pre a))
-      = map ?inst_fmla (pne_equiv_dnf_list (ac_pre a))"
-    using pne_equiv_dnf_list_map[of ?h "ac_pre a"] by (simp add: comp_def)
+  have inst_def: "is_def_explicated_conj (?inst_fmla (ac_pre a))"
+    using is_def_explicated_conj_map_atom_fmla
+          def_explicated_conj_dom[unfolded def_explicated_conj_dom_def] assms by blast
+
+  have map_dnf: "dnf_list (?inst_fmla (ac_pre a))
+      = map ?inst_fmla (dnf_list (ac_pre a))"
+    using dnf_list_map[of "map_atom ?h" "ac_pre a"] by (simp add: comp_def)
 
   have "valuation M \<Turnstile>\<^sub>m ground_action.precondition (instantiate_classical_action_schema a args)
       \<longleftrightarrow> valuation M \<Turnstile>\<^sub>m ?inst_fmla (ac_pre a)"
     by (simp add: pre_eq)
-  also have "... \<longleftrightarrow> (\<exists>c\<in>set (pne_equiv_dnf_list (?inst_fmla (ac_pre a))). valuation M \<Turnstile>\<^sub>m c)"
-    by (rule pne_equiv_dnf_list_map_semantics)
-  also have "... \<longleftrightarrow> (\<exists>c\<in>set (pne_equiv_dnf_list (ac_pre a)). valuation M \<Turnstile>\<^sub>m ?inst_fmla c)"
+  also have "... \<longleftrightarrow> (\<exists>c\<in>set (dnf_list (?inst_fmla (ac_pre a))). valuation M \<Turnstile>\<^sub>m c)"
+    by (rule is_def_explicated_conj_dnf_list_map_semantics[OF inst_def])
+  also have "... \<longleftrightarrow> (\<exists>c\<in>set (dnf_list (ac_pre a)). valuation M \<Turnstile>\<^sub>m ?inst_fmla c)"
     unfolding map_dnf by simp
   also have "... \<longleftrightarrow> (\<exists>a'\<in>set (split_ac a). valuation M \<Turnstile>\<^sub>m ?inst_fmla (ac_pre a'))"
     by (rule precond_prop_iff_split)
@@ -328,35 +280,6 @@ proof -
       valuation M \<Turnstile>\<^sub>m ground_action.precondition (instantiate_classical_action_schema a' args))"
     using a'_pre by metis
   finally show ?thesis .
-qed
-
-
-lemma (in ast_classical_problem4) p_ac_params_match:
-  assumes "a' \<in> set (split_ac a)"
-  shows "action_params_match (head a) = action_params_match (head a')"
-  using split_ac_sel(2)[OF assms] action_params_match_def by presburger
-
-lemma (in ast_classical_problem4) p_effect_same:
-  assumes "b' \<in> set (split_ac b)"
-          "resolve_classical_action_schema n = Some b" 
-          "p4.resolve_classical_action_schema n' = Some b'"
-        shows "effect ((the o res_inst) (SimplePlanAction n args)) = effect ((the o p4.res_inst) (SimplePlanAction n' args))"
-  using instantiate_classical_action_schema_alt
-  using split_ac_sel[OF assms(1)] assms(2-) by auto
-  
-lemma (in ast_classical_problem4) p_exec:
-  assumes "a' \<in> set (split_ac a)"
-    "resolve_classical_action_schema n = Some a" "p4.resolve_classical_action_schema n' = Some a'"
-  shows "execute_plan_action (SimplePlanAction n args) = p4.execute_plan_action (SimplePlanAction n' args)"
-proof -
-  have "effect ((the o res_inst) (SimplePlanAction n args)) = effect ((the o p4.res_inst) (SimplePlanAction n' args))"
-    using assms p_effect_same by simp
-  hence "apply_ground_actions [(the o res_inst) (SimplePlanAction n args)] = 
-    apply_ground_actions [(the o p4.res_inst) (SimplePlanAction n' args)]"
-    using apply_ground_actions_equiv_weak by auto
-  thus ?thesis
-    unfolding ast_classical_problem.execute_plan_action_def 
-    by simp
 qed
 
 end
@@ -369,20 +292,20 @@ lemma split_pa_enabled:
 proof (cases \<pi>)
   case [simp]: (SimplePlanAction n args)
 
-  obtain a where 
-    a: "resolve_classical_action_schema n = Some a" 
+  obtain a where
+    a: "resolve_classical_action_schema n = Some a"
     "action_params_match (head a) args"
     "a \<in> set (actions D)"
-    using plan_action_enabled_props[OF assms] 
+    using plan_action_enabled_props[OF assms]
     using wf_pa_refs_ac by force
 
   have v_pre: "valuation M \<Turnstile>\<^sub>m precondition (instantiate_classical_action_schema a args)"
     using plan_action_enabled_props[OF assms] a by simp
 
-  obtain a' where 
+  obtain a' where
     a': "a' \<in> set (split_ac a)"
     "valuation M \<Turnstile>\<^sub>m precondition (instantiate_classical_action_schema a' args)"
-    using v_pre inst_pre_iff_split by metis
+    using v_pre inst_pre_iff_split[OF a(3)] by metis
 
   let ?pi = "SimplePlanAction n args"
   let ?pi' = "SimplePlanAction (ac_name a') args"
@@ -403,14 +326,14 @@ proof (cases \<pi>)
   (* defined *)
   have effs_same: "effect ((the o res_inst) \<pi>) = effect ((the o p4.res_inst) ?pi')"
     using a' p_effect_same a(1) res' by auto
-  
+
   have "set (ast_effect_enumerate_rhs_primitive_numeric_expressions (effect ((the o res_inst) \<pi>))) \<subseteq> dom (snd M)"
     using assms plan_action_enabled_props by presburger
   hence effs_defined': "set (ast_effect_enumerate_rhs_primitive_numeric_expressions (effect ((the o p4.res_inst) ?pi'))) \<subseteq> dom (snd M)"
     using effs_same by argo
 
   (* non-interfering *)
-  have "numeric_effects_non_intrf ((the o res_inst) \<pi>)" 
+  have "numeric_effects_non_intrf ((the o res_inst) \<pi>)"
     using assms plan_action_enabled_props by blast
   hence non_int': "numeric_effects_non_intrf ((the o p4.res_inst) ?pi')"
     using numeric_effects_non_intrf_def effs_same by auto
@@ -435,14 +358,14 @@ next
     using split_pa_enabled valid_classical_plan_from2_Cons by blast
   obtain \<pi>s' where "p4.valid_classical_plan_from2 (p4.execute_plan_action \<pi>' s) \<pi>s'"
   proof -
-    have "valid_classical_plan_from2 (execute_plan_action \<pi> s) \<pi>s" using Cons(3) 
+    have "valid_classical_plan_from2 (execute_plan_action \<pi> s) \<pi>s" using Cons(3)
       unfolding valid_classical_plan_from2_alt by simp
     hence valid': "valid_classical_plan_from2 (p4.execute_plan_action \<pi>' s) \<pi>s" using pi' by simp
 
     have wf_wm': "p4.wf_world_model s" using Cons by simp
-    
+
     have wf_act': "p4.wf_classical_plan_action \<pi>'" using Cons pi'(1) p4.plan_action_enabled_props by simp
-    have "\<exists>\<pi>s'. p4.valid_classical_plan_from2 (p4.execute_plan_action \<pi>' s) \<pi>s'" 
+    have "\<exists>\<pi>s'. p4.valid_classical_plan_from2 (p4.execute_plan_action \<pi>' s) \<pi>s'"
       apply (rule Cons.IH)
       using  p4_wf.wf_execute_stronger[OF wf_act'] wf_wm' apply simp
       using valid' by blast
@@ -452,9 +375,9 @@ next
     show ?thesis by blast
   qed
   then obtain M' where
-    "p4.valid_classical_plan_alt (p4.execute_plan_action \<pi>' s) \<pi>s' M'" 
+    "p4.valid_classical_plan_alt (p4.execute_plan_action \<pi>' s) \<pi>s' M'"
     "valuation M' \<Turnstile>\<^sub>m goal split_prob" unfolding p4.valid_classical_plan_from2_alt by blast
-  thus ?case unfolding p4.valid_classical_plan_from2_alt 
+  thus ?case unfolding p4.valid_classical_plan_from2_alt
     apply (intro exI)
     apply (subst p4.valid_classical_plan_alt.simps(2))
     using pi'(1) by force
@@ -466,8 +389,8 @@ lemma (in ast_classical_domain4) restore_split_ac:
 proof -
   from assms have "ac_name a' \<in> set (map ac_name (split_ac a))" by auto
   hence "ac_name a' \<in> set (split_ac_names a)"
-    unfolding split_ac_def Let_def
-    using split_ac_names_length pne_equiv_dnf_list_length set_n_pre_mapsel(1) by metis
+    unfolding split_ac_def
+    using split_ac_names_length set_n_pre_mapsel(1) by metis
   thus ?thesis
     using assms split_names_prefix_length drop_lit_prefix by metis
 qed
@@ -567,7 +490,7 @@ proof (induction \<pi>')
     using pre_sat' unfolding comp_def p4.res_inst.simps res'
     unfolding \<pi> unfolding res_inst.simps res
     unfolding option.sel
-    using inst_pre_iff_split
+    using inst_pre_iff_split[OF in_acts]
     using ac_split by blast
 
   show "plan_action_enabled \<pi> M" unfolding plan_action_enabled_def
@@ -579,20 +502,20 @@ lemma restore_plan_split_valid_from:
   shows "valid_classical_plan_from2 s (restore_plan_split \<pi>s')"
 using assms proof (induction \<pi>s' arbitrary: s)
   case Nil thus ?case
-    unfolding ast_classical_problem.valid_classical_plan_from2_alt split_prob_sel 
+    unfolding ast_classical_problem.valid_classical_plan_from2_alt split_prob_sel
     by simp
 next
   case (Cons \<pi>' \<pi>s')
   let ?pis = "restore_plan_split \<pi>s'"
 
-  have enabled: "plan_action_enabled (restore_pa_split \<pi>') s" 
+  have enabled: "plan_action_enabled (restore_pa_split \<pi>') s"
     using Cons restore_pa_enabled by auto
 
-  have wf': "p4.wf_classical_plan_action \<pi>'" using Cons 
+  have wf': "p4.wf_classical_plan_action \<pi>'" using Cons
     unfolding p4.valid_classical_plan_from2_alt
     by (auto intro: p4.plan_action_enabled_props)
 
-  have execute_equiv: "execute_plan_action (restore_pa_split \<pi>') s 
+  have execute_equiv: "execute_plan_action (restore_pa_split \<pi>') s
     = p4.execute_plan_action \<pi>' s"
     apply (rule restore_pa_execute)
     using wf' by presburger
@@ -603,7 +526,7 @@ next
       using p4_wf.wf_execute_stronger[OF wf'] \<open>p4.wf_world_model s\<close>
       using execute_equiv by auto
     show "p4.valid_classical_plan_from2 (execute_plan_action (restore_pa_split \<pi>') s) \<pi>s'"
-      using \<open>p4.valid_classical_plan_from2 s (\<pi>' # \<pi>s')\<close> 
+      using \<open>p4.valid_classical_plan_from2 s (\<pi>' # \<pi>s')\<close>
       unfolding p4.valid_classical_plan_from2_alt using execute_equiv by simp
   qed
   show ?case using valid_classical_plan_from2_Cons enabled valid by simp
@@ -624,8 +547,6 @@ theorem restore_plan_split_valid:
   using restore_plan_split_valid_from wf_I by simp
 
 end
-
-(* under which conditions does the set of defined pnes not change *)
 
 subsection \<open> Code Setup \<close>
 
