Reachability_Analysis.thy
@@ -1,6 +1,9 @@
 theory Reachability_Analysis
-  imports PDDL_Sema_Supplement Normalization_Definitions
-    Formula_Utils Graph_Funs String_Utils
+  imports Tree_Decomp_Grounding_Base.PDDL_Sema_Supplement
+    Tree_Decomp_Grounding_Base.Normalization_Definitions
+    Tree_Decomp_Grounding_Base.Formula_Utils
+    Tree_Decomp_Grounding_Base.Graph_Funs
+    Tree_Decomp_Grounding_Base.String_Utils
     (*"AI_Planning_Languages_Semantics.PDDL_STRIPS_Checker"*)
 begin
 
