Type_Normalization/Type_Normalization_Locales.thy
@@ -1,8 +1,8 @@
 theory Type_Normalization_Locales
   imports "Classical_Planning.Classical_Abstract_Syntax"
-    Tree_Decomp_Grounding.Normalization_Definitions 
-    Tree_Decomp_Grounding.Graph_Funs
-    Tree_Decomp_Grounding.String_Utils iq.iq
+    Tree_Decomp_Grounding_Base.Normalization_Definitions
+    Tree_Decomp_Grounding_Base.Graph_Funs
+    Tree_Decomp_Grounding_Base.String_Utils iq.iq
 begin
 
 section \<open>Type Normalization Definitions and Locales\<close>
