ROOT
@@ -1,48 +1,15 @@
 chapter AFP
 
-session Tree_Decomp_Grounding = HOL +
+session Tree_Decomp_Grounding = Tree_Decomp_Grounding_Base +
   description \<open>An executable grounder for PDDL tasks based on FastDownward system.\<close>
   options [timeout = 900]
   sessions
-	"Classical_Planning"
-	"HOL-Library"
-	"Show"
-	"Propositional_Proof_Systems"
-  theories [document = false]
-	"HOL-Library.Sublist"
-	"HOL-Library.List_Lexorder"
-	"HOL-Library.Char_ord"
-	"HOL-Library.Monad_Syntax"
-	"Show.Show_Instances"
-	"Propositional_Proof_Systems.Sema"
-	"Propositional_Proof_Systems.CNF"
-    "Propositional_Proof_Systems.CNF_Formulas"
-    "Propositional_Proof_Systems.CNF_Sema"
-    "Propositional_Proof_Systems.CNF_Formulas_Sema"
-  theories [document = false]
-    Grounding_Utils
-	Formula_Utils
-	Nat_Show_Utils
-	String_Utils
-	PDDL_Sema_Supplement
-	STRIPS_Sema_Supplement	
-	PDDL_Checker_Utils
+	"Type_Normalization"
+	"Definedness_Normalization"
+	"Goal_Normalization"
+	"Precondition_Normalization"
+	"PDDL_Relaxation"
   theories
-	DNF
-	Graph_Funs
-	Normalization_Definitions
-	"Type_Normalization/Type_Normalization_Locales"
-	"Type_Normalization/Type_Normalization"
-	"Type_Normalization/Type_Normalization_Semantics"
-	"Goal_Normalization/Goal_Normalization_Locales"
-	"Goal_Normalization/Goal_Normalization"
-	"Goal_Normalization/Goal_Normalization_Semantics"
-	"Precondition_Normalization/Precondition_Normalization_Locales"
-	"Precondition_Normalization/Precondition_Normalization"
-	"Precondition_Normalization/Precondition_Normalization_Semantics"
-	"PDDL_Relaxation/PDDL_Relaxation_Locales"
-	"PDDL_Relaxation/PDDL_Relaxation"
-	"PDDL_Relaxation/PDDL_Relaxation_Semantics"
 	Reachability_Analysis
 	Grounded_PDDL
 	PDDL_to_STRIPS
